hmacdrbg/HMAC_DRBG_common_lemmas.v
@@ -6,15 +6,54 @@ Require Import hmacdrbg.hmac_drbg.
 Require Import hmacdrbg.spec_hmac_drbg.
 Require Import sha.general_lemmas.
 
+Lemma da_emp_isptrornull sh t v p :
+   da_emp sh t v p = (!!is_pointer_or_null p) &&  da_emp sh t v p.
+ Proof. unfold da_emp; apply pred_ext.
+  + apply orp_left.
+    - apply derives_extract_prop; intros; subst; simpl. entailer. apply orp_right1. trivial.
+    - rewrite data_at_isptr with (p0:=p) at 1. normalize.
+      destruct p; simpl in *; try contradiction. entailer. apply orp_right2. trivial.
+  + entailer.
+Qed.
+
+Lemma da_emp_null sh t v p: p=nullval -> da_emp sh t v p = emp.
+Proof. intros; subst. unfold da_emp. rewrite data_at_isptr.
+  apply pred_ext.
+  + normalize. rewrite orp_FF. trivial.
+  + simpl. apply orp_right1. entailer.
+Qed. 
+Lemma da_emp_ptr sh t v b i: da_emp sh t v (Vptr b i) = data_at sh t v (Vptr b i).
+Proof. intros; unfold da_emp, nullval; simpl.
+  apply pred_ext.
+  + apply orp_left; trivial. normalize. inv H.
+  + apply orp_right2. trivial.
+Qed.  
+
+Lemma Tarray_0_emp sh v c: data_at sh (Tarray tuchar 0 noattr) v c |--  emp.
+  unfold data_at. unfold field_at, data_at_rec, at_offset; simpl.
+  unfold array_pred, unfold_reptype, aggregate_pred.array_pred. entailer.
+Qed.
+ 
+Lemma Tarray_0_emp' sh c: field_compatible (Tarray tuchar 0 noattr) nil c ->
+  emp |-- data_at sh (Tarray tuchar 0 noattr) nil c.
+Proof. intros.
+  unfold data_at. unfold field_at, data_at_rec, at_offset; simpl.
+  unfold array_pred, unfold_reptype, aggregate_pred.array_pred. simpl.
+  entailer.
+Qed. 
+
 Lemma data_at_weak_valid_ptr: forall (sh : Share.t) (t : type) (v : reptype t) (p : val),
        sepalg.nonidentity sh ->
-       sizeof (*cenv_cs*) t >= 0 -> data_at sh t v p |-- weak_valid_pointer p.
-Proof.
-Admitted.
+       (*sizeof cenv_cs t >= 0 -> *) sizeof t > 0 -> data_at sh t v p |-- weak_valid_pointer p.
+Proof. intros. 
+eapply derives_trans. 2: apply valid_pointer_weak. apply data_at_valid_ptr; trivial. Qed.
+
 Lemma sepcon_weak_valid_pointer2
 : forall (P Q : mpred) (p : val),
     P |-- weak_valid_pointer p -> Q * P |-- weak_valid_pointer p.
-Proof. Admitted.
+Proof.
+intros. unfold weak_valid_pointer in *.
+Admitted.
 Lemma sepcon_weak_valid_pointer1
 : forall (P Q : mpred) (p : val),
     P |-- weak_valid_pointer p -> P * Q |-- weak_valid_pointer p.
